ulib/ml/FStar_UInt_UInt63.ml
@@ -1,0 +1,62 @@
+type uint63 = int
+type uint8 = int
+                
+let (%) x y = if x < 0 then (x mod y) + y else x mod y
+
+let v (x:uint63) : Prims.int = Prims.parse_int (string_of_int x)
+
+let add (a:uint63) (b:uint63) : uint63 = a + b
+let add_underspec a b = add a b
+let add_mod a b = add a b
+
+let sub (a:uint63) (b:uint63) : uint63 = a - b
+let sub_underspec a b = sub a b
+let sub_mod a b = sub a b
+
+let mul (a:uint63) (b:uint63) : uint63 = a * b
+let mul_underspec a b = mul a b
+let mul_mod a b = mul a b
+
+let div (a:uint63) (b:uint63) : uint63 = failwith "Not implemented"
+
+let rem (a:uint63) (b:uint63) : uint63 = failwith "Not implemented"
+
+let logand (a:uint63) (b:uint63) : uint63 = a land b
+let logxor (a:uint63) (b:uint63) : uint63 = a lxor b
+let logor  (a:uint63) (b:uint63) : uint63 = a lor b
+let lognot (a:uint63) : uint63 = lnot a
+       
+let int_to_uint63 (x:Prims.int) : uint63 = int_of_string (Prims.to_string x) 
+
+let shift_right (a:uint63) (b:uint8) : uint63 = a lsr b
+let shift_left  (a:uint63) (b:uint8) : uint63 = (a lsl b)
+
+(* Comparison operators *)
+let eq (a:uint63) (b:uint63) : bool = a = b
+let gt (a:uint63) (b:uint63) : bool = a > b
+let gte (a:uint63) (b:uint63) : bool = a >= b
+let lt (a:uint63) (b:uint63) : bool = a < b
+let lte (a:uint63) (b:uint63) : bool =  a <= b
+
+(* Infix notations *)
+let op_Hat_Plus = add
+let op_Hat_Plus_Question = add_underspec
+let op_Hat_Plus_Percent = add_mod
+let op_Hat_Subtraction = sub
+let op_Hat_Subtraction_Question = sub_underspec
+let op_Hat_Subtraction_Percent = sub_mod
+let op_Hat_Star = mul
+let op_Hat_Star_Question = mul_underspec
+let op_Hat_Star_Percent = mul_mod
+let op_Hat_Slash = div
+let op_Hat_Percent = rem
+let op_Hat_Hat = logxor  
+let op_Hat_Amp = logand
+let op_Hat_Bar = logor
+let op_Hat_Less_Less = shift_left
+let op_Hat_Greater_Greater = shift_right
+let op_Hat_Equal = eq
+let op_Hat_Greater = gt
+let op_Hat_Greater_Equal = gte
+let op_Hat_Less = gt
+let op_Hat_Less_Equal = gte
