ulib/FStar.UInt.fst
@@ -1,22 +1,21 @@
 module FStar.UInt
 
-open FStar.Ghost
+let op_Star = op_Multiply
 
-val pow2: nat -> Tot pos
-let rec pow2 x = if x = 0 then 1 else op_Multiply 2 (pow2 (x-1))
+let rec pow2 (x:nat) : Tot pos = if x = 0 then 1 else 2 * (pow2 (x-1))
 
-type uSize (x:int) (n:nat) = (x >= 0 /\ x < pow2 n)
+let max_int (n:nat) : Tot int = pow2 n - 1
+let min_int (n:nat) : Tot int = 0
+
+let uSize (x:int) (n:nat) : GTot Type0 = (x >= min_int n /\ x <= max_int n)
 
 (* Machine integer type *)
+// JK: note that if used without going through the F* libraries specific submodule that will be 
+// realized as a Bigint
 type uint (n:nat) = x:int{uSize x n}
 
-(* Specs *)
-val max_int: n:nat -> Tot (uint n)
-let max_int n = pow2 n - 1
-
-val min_int: n:nat -> Tot (uint n)
-let min_int n = 0
-
+(* Constants *)
+//let zero n : Tot (uint n) = 0
 val zero: n:nat -> Tot (uint n)
 let zero n = 0
 
@@ -32,9 +31,13 @@ let incr #n a = a + 1
 val pred: #n:pos -> a:uint n{a > min_int n} -> Tot (uint n)
 let pred #n a = a - 1
 
+abstract val incr_underspec: #n:pos -> a:uint n -> Tot (b:uint n{a < max_int n ==> b = a + 1})
+let incr_underspec #n a = if (a < max_int n) then a + 1 else magic()
+abstract val pred_underspec: #n:pos -> a:uint n -> Tot (b:uint n{a > min_int n ==> b = a - 1})
+let pred_underspec #n a = if (a > min_int n) then a - 1 else magic()
+
 val incr_mod: #n:pos -> a:uint n -> Tot (uint n)
 let incr_mod #n a = (a + 1) % (pow2 n)
-
 val pred_mod: #n:pos -> a:uint n -> Tot (uint n)
 let pred_mod #n a = (a - 1) % (pow2 n)
 
@@ -42,8 +45,8 @@ let pred_mod #n a = (a - 1) % (pow2 n)
 val add: #n:nat -> a:uint n -> b:uint n{a + b < pow2 n} -> Tot (uint n)
 let add #n a b = a + b
 
-// opaque val add': #n:nat -> a:uint n -> b:uint n -> Tot (c:uint n{a+b<pow2 n ==> c = a + b})
-// let add' #n a b = if (a + b < pow2 n) then a + b else magic()
+abstract val add_underspec: #n:nat -> a:uint n -> b:uint n -> Tot (c:uint n{a + b < pow2 n ==> c = a + b})
+let add_underspec #n a b = if (a + b < pow2 n) then a + b else magic ()
 
 val add_mod: #n:nat -> uint n -> uint n -> Tot (uint n)
 let add_mod #n a b = (a + b) % (pow2 n)
@@ -51,24 +54,36 @@ let add_mod #n a b = (a + b) % (pow2 n)
 (* Subtraction primitives *)
 val sub: #n:nat -> a:uint n -> b:uint n{a - b >= 0} -> Tot (uint n)
 let sub #n a b = a - b
+
+abstract val sub_underspec: #n:nat -> a:uint n -> b:uint n -> Tot (c:uint n{a - b >= 0 ==> c = a - b})
+let sub_underspec #n a b = if (a - b >= 0) then a - b else magic ()
+
 val sub_mod: #n:nat -> a:uint n -> b:uint n -> Tot (uint n)
 let sub_mod #n a b = (a - b) % (pow2 n)
 
 (* Multiplication primitives *)
-val mul: #n:nat -> a:uint n -> b:uint n{op_Multiply a b < pow2 n} -> Tot (uint n)
-let mul #n a b = op_Multiply a b
+val mul: #n:nat -> a:uint n -> b:uint n{a * b < pow2 n} -> Tot (uint n)
+let mul #n a b = a * b
+
+abstract val mul_underspec: #n:nat -> a:uint n -> b:uint n -> Tot (c:uint n{a * b < pow2 n ==> c = a * b})
+let mul_underspec #n a b = if (a * b < pow2 n) then a * b else magic ()
+
 val mul_mod: #n:nat -> a:uint n -> b:uint n -> Tot (uint n)
-let mul_mod #n a b = (op_Multiply a b) % (pow2 n)
+let mul_mod #n a b = (a * b) % (pow2 n)
 
 (* Division primitives *)
 assume val div: #n:nat -> a:uint n -> b:uint n{b <> 0} -> Tot (c:uint n{c = a / b})
 
-val f: a:nat -> b:nat{b >= 1} -> Lemma (a/b <= a)
-let f a b = ()
-
 (* Modulo primitives *)
 val mod: #n:nat -> a:uint n -> b:uint n{b <> 0} -> Tot (uint n)
-let mod #n a b = a - op_Multiply (a/b) b
+let mod #n a b = a - ((a/b) * b)
+
+(* Comparison operators *)
+let eq #n (a:uint n) (b:uint n) : Tot bool = (a = b)
+let gt #n (a:uint n) (b:uint n) : Tot bool = (a > b)
+let gte #n (a:uint n) (b:uint n) : Tot bool = (a >= b)
+let lt #n (a:uint n) (b:uint n) : Tot bool = (a < b)
+let lte #n (a:uint n) (b:uint n) : Tot bool = (a <= b)
 
 (* Bitwise operators *)
 assume val logand: #n:nat -> uint n -> uint n -> Tot (uint n)
@@ -76,6 +91,7 @@ assume val logxor: #n:nat -> uint n -> uint n -> Tot (uint n)
 assume val logor: #n:nat -> uint n -> uint n -> Tot (uint n)
 assume val lognot: #n:nat -> uint n -> Tot (uint n)
 
+(* JK: bitwise logic should be expressed usint a separate bitvector type *)
 (* Bitwise operators lemmas *)
 assume val logand_lemma_1: #n:nat -> a:uint n -> b:uint n ->
   Lemma (requires True) (ensures ((logand #n a b) = (logand #n b a)))
@@ -115,9 +131,4 @@ let to_uint m a = a % pow2 m
 assume val shift_right: #n:nat -> a:uint n -> s:nat -> Tot (b:uint n{b = a / (pow2 s)})
 
 val shift_left: #n:nat -> a:uint n -> s:nat -> Tot (uint n)
-let shift_left #n a s = (op_Multiply a (pow2 s)) % pow2 n
-
-assume val rotate_left: #n:nat -> a:uint n -> s:nat{s <= n} -> 
-  Tot (b:uint n{b = op_Multiply (a % pow2 (n - s)) (pow2 s) + a / (pow2 (n-s))})
-assume val rotate_right: #n:nat -> a:uint n -> s:nat{s <= n} ->
-  Tot (b:uint n{b = op_Multiply (a % pow2 s) (pow2 (n-s)) + a / pow2 s})
+let shift_left #n a s = (a * (pow2 s)) % pow2 n
