ulib/FStar.Int.Cast.fst
@@ -1,0 +1,188 @@
+module FStar.Int.Cast
+
+module U8  = FStar.UInt.UInt8
+module U16 = FStar.UInt.UInt16
+module U32 = FStar.UInt.UInt32
+module U63 = FStar.UInt.UInt63
+module U64 = FStar.UInt.UInt64
+module I8  = FStar.Int.Int8
+module I16 = FStar.Int.Int16
+module I32 = FStar.Int.Int32
+module I63 = FStar.Int.Int63
+module I64 = FStar.Int.Int64
+
+type u8  = U8.uint8
+type u16 = U16.uint16
+type u32 = U32.uint32
+type u63 = U63.uint63
+type u64 = U64.uint64
+
+type i8  = I8.int8
+type i16 = I16.int16
+type i32 = I32.int32
+type i63 = I63.int63
+type i64 = I64.int64
+
+let op_At_Percent = FStar.Int.op_At_Percent
+
+(** Uints to Uints **)
+assume val uint8_to_uint64: a:u8 -> Tot (b:u64{U64.v b = U8.v a})
+assume val uint8_to_uint63: a:u8 -> Tot (b:u63{U63.v b = U8.v a})
+assume val uint8_to_uint32: a:u8 -> Tot (b:u32{U32.v b = U8.v a})
+assume val uint8_to_uint16: a:u8 -> Tot (b:u16{U16.v b = U8.v a})
+
+assume val uint16_to_uint64: a:u16 -> Tot (b:u64{U64.v b = U16.v a})
+assume val uint16_to_uint63: a:u16 -> Tot (b:u63{U63.v b = U16.v a})
+assume val uint16_to_uint32: a:u16 -> Tot (b:u32{U32.v b = U16.v a})
+//assume val uint16_to_uint8: a:u16 -> Tot (b:u8{b = U8.int_to_uint8 (U16.v a)})
+assume val uint16_to_uint8 : a:u16 -> Tot (b:u8{U8.v b = U16.v a % FStar.UInt.pow2 8})
+
+assume val uint32_to_uint64: a:u32 -> Tot (b:u64{U64.v b = U32.v a})
+assume val uint32_to_uint63: a:u32 -> Tot (b:u63{U63.v b = U32.v a})
+//assume val uint32_to_uint16: a:u32 -> Tot (b:u16{b = U16.int_to_uint16 (U32.v a)})
+//assume val uint32_to_uint8: a:u32 -> Tot (b:u8{b = U8.int_to_uint8 (U32.v a)})
+assume val uint32_to_uint16: a:u32 -> Tot (b:u16{U16.v b = U32.v a % FStar.UInt.pow2 16})
+assume val uint32_to_uint8 : a:u32 -> Tot (b:u8{U8.v b = U32.v a % FStar.UInt.pow2 8})
+
+assume val uint63_to_uint64: a:u63 -> Tot (b:u64{U64.v b = U63.v a})
+//assume val uint63_to_uint32: a:u63 -> Tot (b:u32{b = U32.int_to_uint32 (U63.v a)})
+//assume val uint63_to_uint16: a:u63 -> Tot (b:u16{b = U16.int_to_uint16 (U63.v a)})
+//assume val uint63_to_uint8: a:u63 -> Tot (b:u8{b = U8.int_to_uint8 (U63.v a)})
+assume val uint63_to_uint32: a:u63 -> Tot (b:u32{U32.v b = U63.v a % FStar.UInt.pow2 32})
+assume val uint63_to_uint16: a:u63 -> Tot (b:u16{U16.v b = U63.v a % FStar.UInt.pow2 16})
+assume val uint63_to_uint8 : a:u63 -> Tot (b:u8{U8.v b = U63.v a % FStar.UInt.pow2 8})
+
+//assume val uint64_to_uint63: a:u64 -> Tot (b:u63{U63.v b = U63.int_to_uint63 (U64.v a)})
+//assume val uint64_to_uint32: a:u64 -> Tot (b:u32{U32.v b = U32.int_to_uint32 (U64.v a})
+//assume val uint64_to_uint16: a:u64 -> Tot (b:u16{U16.v b = U16.int_to_uint16 (U64.v a})
+//assume val uint64_to_uint8: a:u64 -> Tot (b:u8{U8.v b = U8.int_to_uint8 (U64.v a})
+assume val uint64_to_uint63: a:u64 -> Tot (b:u63{U63.v b = U64.v a % FStar.UInt.pow2 63})
+assume val uint64_to_uint32: a:u64 -> Tot (b:u32{U32.v b = U64.v a % FStar.UInt.pow2 32})
+assume val uint64_to_uint16: a:u64 -> Tot (b:u16{U16.v b = U64.v a % FStar.UInt.pow2 16})
+assume val uint64_to_uint8 : a:u64 -> Tot (b:u8{U8.v b = U64.v a % FStar.UInt.pow2 8})
+
+(** Ints to Ints **)
+assume val int8_to_int64: a:i8 -> Tot (b:i64{I64.v b = I8.v a})
+assume val int8_to_int63: a:i8 -> Tot (b:i63{I63.v b = I8.v a})
+assume val int8_to_int32: a:i8 -> Tot (b:i32{I32.v b = I8.v a})
+assume val int8_to_int16: a:i8 -> Tot (b:i16{I16.v b = I8.v a})
+
+assume val int16_to_int64: a:i16 -> Tot (b:i64{I64.v b = I16.v a})
+assume val int16_to_int63: a:i16 -> Tot (b:i63{I63.v b = I16.v a})
+assume val int16_to_int32: a:i16 -> Tot (b:i32{I32.v b = I16.v a})
+//assume val int16_to_int8: a:i16 -> Tot (b:u8{b = I8.int_to_int8 (I16.v a)})
+assume val int16_to_int8 : a:i16 -> Tot (b:i8 {I8.v b  = (I16.v a @% FStar.Int.pow2 8)})
+
+assume val int32_to_int64: a:i32 -> Tot (b:i64{I64.v b = I32.v a})
+assume val int32_to_int63: a:i32 -> Tot (b:i63{I63.v b = I32.v a})
+//assume val int32_to_int16: a:i32 -> Tot (b:i16{b = I16.int_to_int16 (I32.v a)})
+//assume val int32_to_int8: a:i32 -> Tot (b:i8{b = I8.int_to_int8 (I32.v a)})
+assume val int32_to_int16: a:i32 -> Tot (b:i16{I16.v b = (I32.v a @% FStar.Int.pow2 16)})
+assume val int32_to_int8 : a:i32 -> Tot (b:i8 {I8.v b  = (I32.v a @% FStar.Int.pow2 8)})
+
+assume val int63_to_int64: a:i63 -> Tot (b:i64{I64.v b = I63.v a})
+//assume val int63_to_int32: a:i63 -> Tot (b:i32{b = I32.int_to_int32 (I63.v a)})
+//assume val int63_to_int16: a:i63 -> Tot (b:i16{b = I16.int_to_int16 (I63.v a)})
+//assume val int63_to_int8: a:i63 -> Tot (b:i8{b = I8.int_to_int8 (I63.v a)})
+assume val int63_to_int32: a:i63 -> Tot (b:i32{I32.v b = (I63.v a @% FStar.Int.pow2 32)})
+assume val int63_to_int16: a:i63 -> Tot (b:i16{I16.v b = (I63.v a @% FStar.Int.pow2 16)})
+assume val int63_to_int8 : a:i63 -> Tot (b:i8 {I8.v b  = (I63.v a @% FStar.Int.pow2 8)})
+
+//assume val int64_to_int63: a:i64 -> Tot (b:i63{I63.v b = I63.int_to_int63 (U64.v a)})
+//assume val int64_to_int32: a:i64 -> Tot (b:i32{I32.v b = U32.int_to_int32 (I64.v a})
+//assume val int64_to_int16: a:i64 -> Tot (b:i16{I16.v b = I16.int_to_int16 (I64.v a})
+//assume val int64_to_int8: a:i64 -> Tot (b:i8{I8.v b = I8.int_to_int8 (I64.v a})
+assume val int64_to_int63: a:i64 -> Tot (b:i63{I63.v b = (I64.v a @% FStar.Int.pow2 63)})
+assume val int64_to_int32: a:i64 -> Tot (b:i32{I32.v b = (I64.v a @% FStar.Int.pow2 32)})
+assume val int64_to_int16: a:i64 -> Tot (b:i16{I16.v b = (I64.v a @% FStar.Int.pow2 16)})
+assume val int64_to_int8 : a:i64 -> Tot (b:i8 {I8.v b  = (I64.v a @% FStar.Int.pow2 8)})
+
+(** Uints to Ints **)
+assume val uint8_to_int64: a:u8 -> Tot (b:i64{I64.v b = U8.v a})
+assume val uint8_to_int63: a:u8 -> Tot (b:i63{I63.v b = U8.v a})
+assume val uint8_to_int32: a:u8 -> Tot (b:i32{I32.v b = U8.v a})
+assume val uint8_to_int16: a:u8 -> Tot (b:i16{I16.v b = U8.v a})
+assume val uint8_to_int8 : a:u8 -> Tot (b:i8 {I8.v b  = (U8.v a @% FStar.Int.pow2 8)})
+
+assume val uint16_to_int64: a:u16 -> Tot (b:i64{I64.v b = U16.v a})
+assume val uint16_to_int63: a:u16 -> Tot (b:i63{I63.v b = U16.v a})
+assume val uint16_to_int32: a:u16 -> Tot (b:i32{I32.v b = U16.v a})
+//assume val uint16_to_int16: a:u16 -> Tot (b:u16{b = I16.int_to_int16 (U16.v a)})
+//assume val uint16_to_int8: a:u16 -> Tot (b:u8{b = I8.int_to_int8 (U16.v a)})
+assume val uint16_to_int16: a:u16 -> Tot (b:i16{I16.v b = (U16.v a @% FStar.Int.pow2 16)})
+assume val uint16_to_int8 : a:u16 -> Tot (b:i8 {I8.v b  = (U16.v a @% FStar.Int.pow2 8)})
+
+assume val uint32_to_int64: a:u32 -> Tot (b:i64{I64.v b = U32.v a})
+assume val uint32_to_int63: a:u32 -> Tot (b:i63{I63.v b = U32.v a})
+//assume val uint32_to_int32: a:u32 -> Tot (b:i32{b = I32.int_to_int32 (U32.v a)})
+//assume val uint32_to_int16: a:u32 -> Tot (b:i16{b = I16.int_to_int16 (U32.v a)})
+//assume val uint32_to_int8: a:u32 -> Tot (b:i8{b = I8.int_to_int8 (U32.v a)})
+assume val uint32_to_int32: a:u32 -> Tot (b:i32{I32.v b = (U32.v a @% FStar.Int.pow2 32)})
+assume val uint32_to_int16: a:u32 -> Tot (b:i16{I16.v b = (U32.v a @% FStar.Int.pow2 16)})
+assume val uint32_to_int8 : a:u32 -> Tot (b:i8 {I8.v b  = (U32.v a @% FStar.Int.pow2 8)})
+
+assume val uint63_to_int64: a:u63 -> Tot (b:i64{I64.v b = U63.v a})
+//assume val uint63_to_int63: a:u63 -> Tot (b:i63{b = I63.int_to_int63 (U63.v a)})
+//assume val uint63_to_int32: a:u63 -> Tot (b:i32{b = I32.int_to_int32 (U63.v a)})
+//assume val uint63_to_int16: a:u63 -> Tot (b:i16{b = I16.int_to_int16 (U63.v a)})
+//assume val uint63_to_int8: a:u63 -> Tot (b:i8{b = I8.int_to_int8 (U63.v a)})
+assume val uint63_to_int63: a:u63 -> Tot (b:i63{I63.v b = (U63.v a @% FStar.Int.pow2 63)})
+assume val uint63_to_int32: a:u63 -> Tot (b:i32{I32.v b = (U63.v a @% FStar.Int.pow2 32)})
+assume val uint63_to_int16: a:u63 -> Tot (b:i16{I16.v b = (U63.v a @% FStar.Int.pow2 16)})
+assume val uint63_to_int8 : a:u63 -> Tot (b:i8 {I8.v b  = (U63.v a @% FStar.Int.pow2 8)})
+
+//assume val uint64_to_int64: a:u64 -> Tot (b:i64{I64.v b = I64.int_to_int64 (U64.v a)})
+//assume val uint64_to_int63: a:u64 -> Tot (b:i63{I63.v b = I63.int_to_int63 (U64.v a)})
+//assume val uint64_to_int32: a:u64 -> Tot (b:i32{I32.v b = U32.int_to_int32 (U64.v a})
+//assume val uint64_to_int16: a:u64 -> Tot (b:i16{I16.v b = I16.int_to_int16 (U64.v a})
+//assume val uint64_to_int8: a:u64 -> Tot (b:i8{I8.v b = I8.int_to_int8 (U64.v a})
+assume val uint64_to_int64: a:u64 -> Tot (b:i64{I64.v b = (U64.v a @% FStar.Int.pow2 64)})
+assume val uint64_to_int63: a:u64 -> Tot (b:i63{I63.v b = (U64.v a @% FStar.Int.pow2 63)})
+assume val uint64_to_int32: a:u64 -> Tot (b:i32{I32.v b = (U64.v a @% FStar.Int.pow2 32)})
+assume val uint64_to_int16: a:u64 -> Tot (b:i16{I16.v b = (U64.v a @% FStar.Int.pow2 16)})
+assume val uint64_to_int8 : a:u64 -> Tot (b:i8 {I8.v b  = (U64.v a @% FStar.Int.pow2 8)})
+
+(** Ints to uints *)
+assume val int8_to_uint64: a:i8 -> Tot (b:u64{U64.v b = I8.v a % FStar.UInt.pow2 64})
+assume val int8_to_uint63: a:i8 -> Tot (b:u63{U63.v b = I8.v a % FStar.UInt.pow2 63})
+assume val int8_to_uint32: a:i8 -> Tot (b:u32{U32.v b = I8.v a % FStar.UInt.pow2 32})
+assume val int8_to_uint16: a:i8 -> Tot (b:u16{U16.v b = I8.v a % FStar.UInt.pow2 16})
+assume val int8_to_uint8 : a:i8 -> Tot (b:u8 {U8.v b  = I8.v a % FStar.UInt.pow2 8})
+
+assume val int16_to_uint64: a:i16 -> Tot (b:u64{U64.v b = I16.v a % FStar.UInt.pow2 64})
+assume val int16_to_uint63: a:i16 -> Tot (b:u63{U63.v b = I16.v a % FStar.UInt.pow2 63})
+assume val int16_to_uint32: a:i16 -> Tot (b:u32{U32.v b = I16.v a % FStar.UInt.pow2 32})
+assume val int16_to_uint16: a:i16 -> Tot (b:u16{U16.v b = I16.v a % FStar.UInt.pow2 16})
+//assume val int16_to_uint16: a:i16 -> Tot (b:u16{b = U16.int_to_uint16 (I16.v a)})
+//assume val int16_to_uint8: a:i16 -> Tot (b:u8{b = U8.int_to_uint8 (I16.v a)})
+assume val int16_to_uint8 : a:i16 -> Tot (b:u8 {U8.v b  = I16.v a % FStar.UInt.pow2 8})
+
+assume val int32_to_uint64: a:i32 -> Tot (b:u64{U64.v b = I32.v a % FStar.UInt.pow2 64})
+assume val int32_to_uint63: a:i32 -> Tot (b:u63{U63.v b = I32.v a % FStar.UInt.pow2 63})
+assume val int32_to_uint32: a:i32 -> Tot (b:u32{U32.v b = I32.v a % FStar.UInt.pow2 32})
+//assume val int32_to_uint32: a:i32 -> Tot (b:u32{b = U32.int_to_uint32 (I32.v a)})
+//assume val int32_to_uint16: a:i32 -> Tot (b:u16{b = U16.int_to_uint16 (I32.v a)})
+//assume val int32_to_uint8: a:i32 -> Tot (b:u8{b = U8.int_to_uint8 (I32.v a)})
+assume val int32_to_uint16: a:i32 -> Tot (b:u16{U16.v b = I32.v a % FStar.UInt.pow2 16})
+assume val int32_to_uint8 : a:i32 -> Tot (b:u8 {U8.v b  = I32.v a % FStar.UInt.pow2 8})
+
+assume val int63_to_uint64: a:i63 -> Tot (b:u64{U64.v b = I63.v a % FStar.UInt.pow2 64})
+assume val int63_to_uint63: a:i63 -> Tot (b:u63{U63.v b = I63.v a % FStar.UInt.pow2 63})
+//assume val int63_to_uint63: a:i63 -> Tot (b:u63{b = U63.int_to_uint63 (I63.v a)})
+//assume val int63_to_uint32: a:i63 -> Tot (b:u32{b = U32.int_to_uint32 (I63.v a)})
+//assume val int63_to_uint16: a:i63 -> Tot (b:u16{b = U16.int_to_uint16 (I63.v a)})
+//assume val int63_to_uint8: a:i63 -> Tot (b:u8{b = U8.int_to_uint8 (I63.v a)})
+assume val int63_to_uint32: a:i63 -> Tot (b:u32{U32.v b = I63.v a % FStar.UInt.pow2 32})
+assume val int63_to_uint16: a:i63 -> Tot (b:u16{U16.v b = I63.v a % FStar.UInt.pow2 16})
+assume val int63_to_uint8 : a:i63 -> Tot (b:u8 {U8.v b  = I63.v a % FStar.UInt.pow2 8})
+
+//assume val int64_to_uint64: a:i64 -> Tot (b:u64{U64.v b = U64.int_to_uint63 (I64.v a)})
+//assume val int64_to_uint63: a:i64 -> Tot (b:u63{U63.v b = U63.int_to_uint63 (I64.v a)})
+//assume val int64_to_uint32: a:i64 -> Tot (b:u32{U32.v b = U32.int_to_uint32 (I64.v a})
+//assume val int64_to_uint16: a:i64 -> Tot (b:u16{U16.v b = U16.int_to_uint16 (I64.v a})
+//assume val int64_to_uint8: a:i64 -> Tot (b:u8{U8.v b = U8.int_to_uint8 (I64.v a})
+assume val int64_to_uint64: a:i64 -> Tot (b:u64{U64.v b = I64.v a % FStar.UInt.pow2 64})
+assume val int64_to_uint63: a:i64 -> Tot (b:u63{U63.v b = I64.v a % FStar.UInt.pow2 63})
+assume val int64_to_uint32: a:i64 -> Tot (b:u32{U32.v b = I64.v a % FStar.UInt.pow2 32})
+assume val int64_to_uint16: a:i64 -> Tot (b:u16{U16.v b = I64.v a % FStar.UInt.pow2 16})
+assume val int64_to_uint8 : a:i64 -> Tot (b:u8 {U8.v b  = I64.v a % FStar.UInt.pow2 8})
