ulib/FStar.Int.fst
@@ -1,0 +1,122 @@
+module FStar.Int
+
+let op_Star = op_Multiply
+
+(* Necessary mathematical functions *)
+// Powers of n
+let rec pow2 (x:nat) : Tot pos = if x = 0 then 1 else op_Multiply 2 (pow2 (x-1))
+// Absolute value
+let abs (x:int) : Tot int = if x >= 0 then x else -x
+// 'flooring' division
+let op_Slash (a:int) (b:int{b <> 0}) : Tot int = 
+  if (a >= 0 && b < 0) || (a < 0 && b >= 0) then - (abs a / abs b)
+  else abs a / abs b
+// Euclidian division
+let div_eucl (a:int) (b:nonzero) : Tot int =  if a < 0 then (if a % b = 0 then -(-a/b) else -(-a/b) -1) else a / b
+let op_Slash_Percent = div_eucl
+// 'Circular modulo operator : wraps into [-p/2; p/2[
+let op_At_Percent (v:int) (p:int{p>0/\ p%2=0}) : Tot int = let m = v % p in if m >= p/2 then m - p else m
+
+(* Specs *)
+let max_int (n:pos) : Tot int = pow2 (n-1) - 1
+let min_int (n:pos) : Tot int = - (pow2 (n-1))
+
+let fits (x:int) (n:pos) : Tot bool = (min_int n <= x && x <= max_int n)
+let size (x:int) (n:pos) : Tot Type0 = b2t(fits x n)
+type int_t (n:pos) = x:int{size x n}
+
+(* OxO0, 0x01 and 0xf.....f constants *)
+// JK: doesn't work
+// let zero (n:pos) : Tot (int_t n) = 0
+
+val zero: n:pos -> Tot (int_t n)
+let zero n = 0
+
+val one: n:nat{n > 1} -> Tot (int_t n)
+let one n = 1
+
+val ones: n:nat{n > 1} -> Tot (int_t n)
+let ones n = -1
+
+(* Increment and decrement *)
+val incr: #n:pos -> a:int_t n{a < max_int n} -> Tot (int_t n)
+let incr #n a = a + 1
+val pred: #n:pos -> a:int_t n{a > min_int n} -> Tot (int_t n)
+let pred #n a = a - 1
+
+abstract val incr_underspec: #n:pos -> a:int_t n -> Tot (b:int_t n{a < max_int n ==> b = a + 1})
+let incr_underspec #n a = if (a < max_int n) then a + 1 else magic()
+abstract val pred_underspec: #n:pos -> a:int_t n -> Tot (b:int_t n{a > min_int n ==> b = a - 1})
+let pred_underspec #n a = if (a > min_int n) then a - 1 else magic()
+
+val incr_mod: #n:pos -> a:int_t n -> Tot (int_t n)
+let incr_mod #n a = (a + 1) @% (pow2 n)
+val pred_mod: #n:pos -> a:int_t n -> Tot (int_t n)
+let pred_mod #n a = (a - 1) @% (pow2 n)
+
+(* Addition primitives *)
+val add: #n:pos -> a:int_t n -> b:int_t n{size (a + b) n} -> Tot (int_t n)
+let add #n a b = a + b
+
+//let add' #n (a:int_t n) (b:int_t n{a + b < pow2 n}) : Tot (int_t n) = a + b
+//let add #n a b = a + b
+
+abstract val add_underspec: #n:pos -> a:int_t n -> b:int_t n -> 
+  Tot (c:int_t n{size (a+b) n ==> c = a + b})
+let add_underspec #n a b = if fits (a+b) n then a + b else magic ()
+
+val add_mod: #n:pos -> int_t n -> int_t n -> Tot (int_t n)
+let add_mod #n a b = (a + b) @% (pow2 n)
+
+(* Subtraction primitives *)
+val sub: #n:pos -> a:int_t n -> b:int_t n{size (a-b) n} -> Tot (int_t n)
+let sub #n a b = a - b
+
+abstract val sub_underspec: #n:pos -> a:int_t n -> b:int_t n -> 
+  Tot (c:int_t n{size (a-b) n ==> c = a - b})
+let sub_underspec #n a b = if fits (a-b) n then a - b else magic ()
+
+val sub_mod: #n:pos -> a:int_t n -> b:int_t n -> Tot (int_t n)
+let sub_mod #n a b = (a - b) @% (pow2 n)
+
+(* Multiplication primitives *)
+val mul: #n:pos -> a:int_t n -> b:int_t n{size (a*b) n} -> Tot (int_t n)
+let mul #n a b = a * b
+
+abstract val mul_underspec: #n:pos -> a:int_t n -> b:int_t n -> 
+  Tot (c:int_t n{size (a * b) n ==> c = a * b})
+let mul_underspec #n a b = if (fits (a*b) n) then a * b else magic ()
+
+val mul_mod: #n:pos -> a:int_t n -> b:int_t n -> Tot (int_t n)
+let mul_mod #n a b = (a * b) @% (pow2 n)
+
+(* Division primitives *)
+assume val div: #n:pos -> a:int_t n -> b:int_t n{b <> 0} -> Tot (c:int_t n{c = a / b})
+
+(* Modulo primitives *)
+// JK: takes time
+val mod: #n:pos -> a:int_t n -> b:int_t n{b <> 0} -> Tot (int_t n)
+let mod #n a b = a - ((a/b) * b)
+
+(* Bitwise operators *)
+assume val logand: #n:pos -> int_t n -> int_t n -> Tot (int_t n)
+assume val logxor: #n:pos -> int_t n -> int_t n -> Tot (int_t n)
+assume val logor: #n:pos -> int_t n -> int_t n -> Tot (int_t n)
+assume val lognot: #n:pos -> int_t n -> Tot (int_t n)
+
+(* Comparison operators *)
+let eq #n (a:int_t n) (b:int_t n) : Tot bool = (a = b)
+let gt #n (a:int_t n) (b:int_t n) : Tot bool = (a > b)
+let gte #n (a:int_t n) (b:int_t n) : Tot bool = (a >= b)
+let lt #n (a:int_t n) (b:int_t n) : Tot bool = (a < b)
+let lte #n (a:int_t n) (b:int_t n) : Tot bool = (a <= b)
+
+(* Casts *)
+val to_int_t: m:pos -> a:int -> Tot (int_t m)
+let to_int_t m a = a @% pow2 m
+
+(* Shift operators *)
+assume val shift_right: #n:pos -> a:int_t n -> s:nat -> Tot (b:int_t n{b = (a /% (pow2 s))})
+
+val shift_left: #n:pos -> a:int_t n -> s:nat -> Tot (int_t n)
+let shift_left #n a s = (a * (pow2 s)) @% (pow2 n)
