ulib/FStar.UInt.UInt16.fst
@@ -1,0 +1,86 @@
+module FStar.UInt.UInt16
+
+open FStar.UInt
+
+let n = 16
+
+abstract type uint16 = | MkUInt16: v:uint 16 -> uint16
+
+let v (x:uint16) : Tot (x':int{uSize x' n}) = x.v
+
+val add: a:uint16 -> b:uint16{v a + v b < max_int n} -> Tot uint16
+let add a b = MkUInt16 (add (v a) (v b))
+val add_underspec: a:uint16 -> b:uint16 -> Tot uint16
+let add_underspec a b = MkUInt16 (add_underspec #n a.v b.v)
+val add_mod: uint16 -> uint16 -> Tot uint16
+let add_mod a b = MkUInt16 (add_mod #n (v a) (v b))
+val sub: a:uint16 -> b:uint16{v a - v b >= 0} -> Tot uint16
+let sub a b = MkUInt16 (sub (v a) (v b))
+val sub_underspec: a:uint16 -> b:uint16 -> Tot uint16
+let sub_underspec a b = MkUInt16 (sub_underspec (v a) (v b))
+val sub_mod: a:uint16 -> b:uint16 -> Tot uint16
+let sub_mod a b = MkUInt16 (sub_mod (v a) (v b))
+val mul: a:uint16 -> b:uint16{v a * v b < pow2 n} -> Tot uint16
+let mul a b = MkUInt16(mul (v a) (v b))
+val mul_underspec: a:uint16 -> b:uint16 -> Tot uint16
+let mul_underspec a b = MkUInt16(mul_underspec (v a) (v b))
+val mul_mod: a:uint16 -> b:uint16 -> Tot uint16
+let mul_mod a b = MkUInt16 (mul_mod (v a) (v b))
+
+(* Division primitives *)
+val div: a:uint16 -> b:uint16{v b <> 0} -> Tot uint16
+let div a b = MkUInt16(div (v a) (v b))
+
+(* Modulo primitives *)
+val mod: a:uint16 -> b:uint16{v b <> 0} -> Tot uint16
+let mod a b = MkUInt16 (mod (v a) (v b))
+
+(* Bitwise operators *)
+val logand: uint16 -> uint16 -> Tot uint16
+let logand a b = MkUInt16 (logand (v a) (v b))
+val logxor: uint16 -> uint16 -> Tot uint16
+let logxor a b = MkUInt16 (logxor (v a) (v b))
+val logor: uint16 -> uint16 -> Tot uint16
+let logor a b = MkUInt16 (logor (v a) (v b))
+val lognot: uint16 -> Tot uint16
+let lognot a = MkUInt16 (lognot (v a))
+
+val int_to_uint16: x:int -> Tot uint16
+let int_to_uint16 x = MkUInt16 (to_uint 16 x)
+
+(* Shift operators *)
+val shift_right: a:uint16 -> s:nat -> Tot uint16
+let shift_right a s = MkUInt16 (shift_right (v a) s)
+
+val shift_left: a:uint16 -> s:nat -> Tot uint16
+let shift_left a s = MkUInt16 (shift_left (v a) s)
+
+(* Comparison operators *)
+let eq (a:uint16) (b:uint16) : Tot bool = (eq #n (v a) (v b))
+let gt (a:uint16) (b:uint16) : Tot bool = (gt #n (v a) (v b))
+let gte (a:uint16) (b:uint16) : Tot bool = (gte #n (v a) (v b))
+let lt (a:uint16) (b:uint16) : Tot bool = (lt #n (v a) (v b))
+let lte (a:uint16) (b:uint16) : Tot bool = (lte #n (v a) (v b))
+
+(* Infix notations *)
+let op_Hat_Plus = add
+let op_Hat_Plus_Question = add_underspec
+let op_Hat_Plus_Percent = add_mod
+let op_Hat_Subtraction = sub
+let op_Hat_Subtraction_Question = sub_underspec
+let op_Hat_Subtraction_Percent = sub_mod
+let op_Hat_Star = mul
+let op_Hat_Star_Question = mul_underspec
+let op_Hat_Star_Percent = mul_mod
+let op_Hat_Slash = div
+let op_Hat_Percent = mod
+let op_Hat_Hat = logxor  
+let op_Hat_Amp = logand
+let op_Hat_Bar = logor
+let op_Hat_Less_Less = shift_left
+let op_Hat_Greater_Greater = shift_right
+let op_Hat_Equal = eq
+let op_Hat_Greater = gt
+let op_Hat_Greater_Equal = gte
+let op_Hat_Less = gt
+let op_Hat_Less_Equal = gte
